src/Evidence_Bundlers.v
@@ -1,0 +1,31 @@
+Require Import ConcreteEvidence.
+
+Require Import List.
+Import ListNotations.
+
+(* Matches on evidence type param only for verification.  
+   Will extract to the cons function over the first two params (new measurement bits + existing evidence) *)
+Definition cons_uu (x:BS) (e:EvC) (params:ASP_PARAMS) (mpl:Plc) : EvC :=
+  match e with
+  | evc bits et => evc (x :: bits) (uu params mpl et)
+  end.
+
+Definition cons_sig (sig:BS) (e:EvC) (p:Plc): EvC :=
+  match e with
+  | evc bits et => evc (sig :: bits) (gg p et)
+  end.
+
+Definition cons_hh (hsh:BS) (e:EvC) (p:Plc): EvC :=
+  match e with
+  | evc _ et => evc [hsh] (hh p et)
+  end.
+
+Definition ss_cons (e1:EvC) (e2:EvC): EvC :=
+  match (e1, e2) with
+  | (evc bits1 et1, evc bits2 et2) => evc (bits1 ++ bits2) (ss et1 et2)
+  end.
+
+Definition pp_cons (e1:EvC) (e2:EvC): EvC :=
+  match (e1, e2) with
+  | (evc bits1 et1, evc bits2 et2) => evc (bits1 ++ bits2) (pp et1 et2)
+  end.
