src/IO_Stubs.v
@@ -1,0 +1,16 @@
+Require Import Term_Defs.
+
+Definition do_asp (params :ASP_PARAMS) (mpl:Plc) (x:Event_ID) : BS.
+Admitted.
+
+Definition encodeEvRaw(e:RawEv): BS.
+Admitted.
+
+Definition do_sig (bs:BS) (p:Plc) (sigTag:Event_ID) : BS.
+Admitted.
+
+Definition do_hash (bs:BS) (p:Plc) : BS.
+Admitted.
+
+Definition do_start_par_threadIO (loc:Loc) (t:Term) (e:RawEv) : unit.
+Admitted.
