src/VmSemantics.v
@@ -4,8 +4,8 @@ Proofs about the Copland Virtual Machine implementation, linking it to the Copla
 Author:  Adam Petz, ampetz@ku.edu
 *)
 
-Require Import More_lists Defs Term_Defs Term ConcreteEvidence LTS Event_system Term_system Main Appraisal_Evidence.
-Require Import GenStMonad MonadVM Maps StructTactics Auto.
+Require Import More_lists Defs Term_Defs Term ConcreteEvidence LTS Event_system Term_system Main Appraisal_Evidence AutoPrim.
+Require Import MonadVM StructTactics Auto.
 Require Import Axioms_Io Impl_vm External_Facts Helpers_VmSemantics.
 
 Require Import List.
